migrations/sqlite/20260824120000_authentication_oauth.down.sql
@@ -1,0 +1,5 @@
+DROP TABLE IF EXISTS auth_oauth_refresh_tokens;
+DROP TABLE IF EXISTS auth_oauth_access_tokens;
+DROP TABLE IF EXISTS auth_oauth_codes;
+DROP TABLE IF EXISTS auth_oauth_documents;
+DROP TABLE IF EXISTS auth_oauth_clients;
